Code/Syntax/Signature.v
@@ -110,5 +110,5 @@ Module AFSNotation.
              (t1 t2 : tm X C A)
     := RewritingSystem.rew lhs rhs t1 t2.
 
-  Notation "t1 ∼> t2" := (rew _ t1 t2) (at level 70).
+  Notation "t1 ∼> t2" := (rew _ t1 t2) (at level 70). (* \sim is used *)
 End AFSNotation.
